* Optimal Tomita grammars
** Tomita 1
Minimal regular grammar:
#+begin_example
A = 'a'A | epsilon
#+end_example

Minimal regular expression:
#+begin_example
a*
#+end_example

** Tomita 2
Minimal regular grammar:
#+begin_example
A = 'a'B
B = 'b'C
C = 'a'B | epsilon
#+end_example

Minimal regular expression:
#+begin_example
(ab)*
#+end_example

** Tomita 3
Minimal regular grammar:
#+begin_example
A = 'b'A | 'a'B | epsilon
B = 'a'A | 'b'C | epsilon
C = 'b'D
D = 'b'C | 'a'D | epsilon
#+end_example

Minimal regular expression:
#+begin_example
b*(((aa)+b*)|(a(aa)*(bb)+))*a?
#+end_example

** Tomita 4
Minimal regular grammar:
#+begin_example
A = 'a'A | 'b'B | epsilon
B = 'a'A | 'b'C | epsilon
C = 'a'A | epsilon
#+end_example

Minimal regular expression:
#+begin_example
(a|ba|bba)*(bb|b)?
#+end_example

** Tomita 5
Minimal regular grammar:
#+begin_example
A = 'a'D | 'b'B | epsilon
B = 'b'A | 'a'C
C = 'a'B | 'b'D
D = 'b'C | 'a'A
#+end_example

Minimal regular expression:
#+begin_example
(aa|bb|(ab|ba)(aa|bb)*(ab|ba))*
#+end_example

** Tomita 6
Minimal regular grammar:
#+begin_example
A = 'b'B | 'a'C | epsilon
B = 'b'C | 'a'A
C = 'b'A | 'a'B
#+end_example

Minimal regular expression:
#+begin_example
(ba|(a|bb)(ab)*(b|aa))*
#+end_example

** Tomita 7
Minimal regular grammar:
#+begin_example
A = 'b'A | 'a'B | epsilon
B = 'a'B | 'b'C | epsilon
C = 'b'C | 'a'D | epsilon
D = 'a'D | epsilon
#+end_example

Minimal regular expression:
#+begin_example
b*a*b*a*
#+end_example
